src/asn1/RIoT.Ext.fst
@@ -1,25 +1,10 @@
-module ASN1.Low.TLV.Specialized
-
-open ASN1.Base
-
-open ASN1.Spec.Tag
-open ASN1.Spec.Length
-open ASN1.Spec.BOOLEAN
-open ASN1.Spec.NULL
-open ASN1.Spec.OCTET_STRING
-open ASN1.Spec.SEQUENCE
-open ASN1.Spec.TLV.Specialized
+module RIoT.Ext
 
 open LowParse.Low.Base
 open LowParse.Low.Combinators
 
-open ASN1.Low.Base
-open ASN1.Low.Tag
-open ASN1.Low.Length
-open ASN1.Low.BOOLEAN
-open ASN1.Low.NULL
-open ASN1.Low.OCTET_STRING
-open ASN1.Low.SEQUENCE
+open ASN1.Spec
+open ASN1.Low
 
 module U8 = FStar.UInt8
 module U32 = FStar.UInt32
@@ -30,58 +15,6 @@ module B = LowStar.Buffer
 module Cast = FStar.Int.Cast
 
 open FStar.Integers
-
-#reset-options "--query_stats"
-
-/// TODO: Move to spec
-let asn1_length_inbound_of_primitive_value
-  (#_a: asn1_primitive_type)
-  (value: datatype_of_asn1_type _a)
-: GTot (b: bool { b == asn1_length_inbound_of_type _a (length_of_asn1_primitive_value value) })
-= let min, max = asn1_length_bound_of_type _a in
-  let length = length_of_asn1_primitive_value value in
-  asn1_length_inbound length min max
-
-let asn1_length_inbound_of_primitive_TLV
-  (#_a: asn1_primitive_type)
-  (value: datatype_of_asn1_type _a)
-: GTot (b: bool)
-= let min, max = asn1_length_bound_of_type _a in
-  let length = length_of_asn1_primitive_TLV value in
-  asn1_length_inbound length asn1_length_min asn1_length_max
-
-/// Interface
-///
-let serialize32_asn1_TLV_backwards_of_type
-  (_a: asn1_primitive_type)
-: serializer32_backwards (serialize_asn1_TLV_of_type _a)
-= match _a with
-  | BOOLEAN      -> serialize32_asn1_boolean_TLV_backwards ()
-  | NULL         -> serialize32_asn1_null_TLV_backwards ()
-  | OCTET_STRING -> serialize32_asn1_octet_string_TLV_backwards ()
-
-/// Example
-///
-
-/// Extension definition
-
-
-let valid_sequence_value_of
-  (#k: parser_kind)
-  (#t: Type0)
-  (#p: parser k t)
-  (s: serializer p)
-= x: t{ asn1_length_inbound_of_type SEQUENCE (Seq.length (serialize s x)) }
-
-let valid_sequence_len_of
-  (#k: parser_kind)
-  (#t: Type0)
-  (#p: parser k t)
-  (s: serializer p)
-  (x: t)
-= len: asn1_int32_of_type SEQUENCE { v len == Seq.length (serialize s x) }
-
-(*)
 
 noeq
 type algorithmIdentifier_t = {
@@ -153,6 +86,13 @@ let serialize32_algorithmIdentifier_sequence_backwards
 = serialize32_asn1_sequence_TLV_backwards
   (* ls *) (serialize32_algorithmIdentifier_value)
   (*flen*) (len_of_algorithmIdentifier_t_inbound)
+
+// let main ()
+// : HST.ST C.exit_code
+//   (requires fun h -> True)
+//   (ensures fun _ _ _ -> True)
+// =
+//   C.EXIT_SUCCESS
 
 /////////////////////////////////
 noeq
@@ -303,14 +243,14 @@ let serialize32_fwid_sequence
   (*flen*) (len_of_fwid_t_inbound)
 
 //////////////////////////////////
-#push-options "--lax"
+// #push-options "--lax"
 noeq
 type compositeDeviceID_t = {
   version : datatype_of_asn1_type OCTET_STRING; (* INTEGER (1) *)
   deviceID: subjectPublicKeyInfo_t_valid; (* FIXME: F* got stuck here *)
   fwid    : fwid_t_valid
 }
-#pop-options
+// #pop-options
 let compositeDeviceID_t' = ((datatype_of_asn1_type OCTET_STRING & subjectPublicKeyInfo_t_valid) & fwid_t_valid)
 
 let synth_compositeDeviceID_t
@@ -388,12 +328,14 @@ let serialize32_compositeDeviceID_sequence
   (*flen*) (len_of_compositeDeviceID_t_inbound)
 
 /////////////////////////////////////
+#push-options "--lax" (* FIXME *)
 noeq
 type ext_t = {
   riot_oid         : datatype_of_asn1_type OCTET_STRING;
   (* NOTE: ENVELOPING OCTETSTRING? *)
   compositeDeviceID: compositeDeviceID_t_valid;
 }
+#pop-options
 let ext_t' = (datatype_of_asn1_type OCTET_STRING & compositeDeviceID_t_valid)
 
 let synth_ext_t
@@ -460,210 +402,3 @@ let serialize32_ext_sequence
 = serialize32_asn1_sequence_TLV_backwards
   (* ls *) (serialize32_ext_value)
   (*flen*) (len_of_ext_t_inbound)
-
-(*)
-/// Len computing functions for this extension
-///
-#push-options "--query_stats --z3rlimit 4"
-
-let length_of_inner_t_value
-  (x: inner_t)
-: GTot (nat)
-= Seq.length (serialize serialize_inner_value x)
-
-let len_of_inner_t_unbounded
-  (x: inner_t)
-: Tot (len: option (asn1_int32_of_type SEQUENCE) {
-  Some? len ==>
-    v (Some?.v len) == Seq.length (serialize serialize_inner_value x)
-})
-= (* Prf*) serialize_inner_value_unfold x;
-  let len_n1 = len_of_asn1_primitive_TLV_unbounded x.n1 in
-  let len_s1 = len_of_asn1_primitive_TLV_unbounded x.s1 in
-(* retuen *) len_n1 `safe_add` len_s1
-
-let len_of_inner_t_inbound
-  (x: inner_t { asn1_length_inbound_of_type SEQUENCE (Seq.length (serialize serialize_inner_value x)) } )
-: Tot (len: asn1_int32_of_type SEQUENCE {
-  v len == Seq.length (serialize serialize_inner_value x)
-})
-= (* Prf *) serialize_inner_value_unfold x;
-  let len_n1 = len_of_asn1_primitive_TLV_inbound x.n1 in
-  let len_s1 = len_of_asn1_primitive_TLV_inbound x.s1 in
-(* return *) len_n1 + len_s1
-#pop-options
-
-let synth_inner_t_inverse_impl
-  (x: inner_t)
-: Tot (x': inner_t'{x' == synth_inner_t_inverse x})
-= (x.n1, x.s1)
-
-let serialize32_inner_value_backwards ()
-: Tot (serializer32_backwards serialize_inner_value)
-= serialize32_synth_backwards
-  (* s32*) (serialize32_asn1_TLV_backwards_of_type NULL
-            `serialize32_nondep_then_backwards`
-            serialize32_asn1_TLV_backwards_of_type OCTET_STRING)
-  (* f1 *) (synth_inner_t)
-  (* g1 *) (synth_inner_t_inverse)
-  (* g1'*) (synth_inner_t_inverse_impl)
-  (* prf*) ()
-
-let serialize32_inner_sequence_backwards
-= serialize32_asn1_sequence_TLV_backwards
-  (* s32*) (serialize32_inner_value_backwards ())
-  (* len*) (len_of_inner_t_inbound)
-
-/// TEST
-///
-open FStar.Tactics
-
-#restart-solver
-#push-options "--query_stats --z3rlimit 64"
-let inner_t_serialization_test
-  ()
-: HST.Stack unit
-  (requires fun h -> True)
-  (ensures fun h0 _ h1 -> True)
-= HST.push_frame ();
-
-  (* NOTE: Allocate a destination buffer. *)
-  let dst_len = 50ul in
-  let dst = B.alloca 0uy dst_len in
-  let pos = dst_len in
-
-  (* NOTE: Prove writability for buffer with trivial preorder. *)
-  (* Prf *) let h0 = HST.get () in
-  (* Prf *) writable_intro
-            (* buf *) dst
-            (*range*) 0 (B.length dst)
-            (* mem *) h0
-            (* prf *) () (fun s1 s2 -> ());
-
-  (* NOTE: Define an extension instance `x`. *)
-  let n: datatype_of_asn1_type NULL = () in
-  let s: datatype_of_asn1_type OCTET_STRING = (|5ul, Seq.create 5 1uy|) in
-  let x: inner_t = {n1 = n; s1 = s} in
-
-  (* NOTE: Reason about the size of these extension instance `x`. *)
-  (* TODO: We definitely should simplify these spec lemmas. *)
-  (* Prf *) serialize_inner_value_unfold x;
-
-  (* Prf *) serialize_asn1_null_TLV_unfold n;
-  (* Prf *) parser_kind_prop_equiv parse_asn1_null_TLV_kind parse_asn1_null_TLV;
-  (* Prf *) assert (length_of_asn1_primitive_TLV n == 2);
-
-  (* Prf *) serialize_asn1_octet_string_TLV_unfold s;
-  (* Prf *) serialize_the_asn1_tag_unfold OCTET_STRING OCTET_STRING;
-  (* Prf *) serialize_asn1_length_unfold 5ul;
-  (* Prf *) serialize_asn1_octet_string_V_unfold (parser_tag_of_octet_string s) s;
-  (* Prf *) serialize_asn1_octet_string_unfold (v (dfst s)) s;
-  (* Prf *) assert (length_of_asn1_primitive_TLV s == 1 + v (len_of_asn1_length 5ul) + 5);
-
-  (* Prf *) serialize_inner_sequence_unfold x;
-  (* Prf *) serialize_asn1_sequence_TL_unfold (parser_tag_of_asn1_sequence serialize_inner_value x);
-  (* Prf *) serialize_the_asn1_tag_unfold SEQUENCE SEQUENCE;
-  (* Prf *) serialize_asn1_length_unfold (len_of_asn1_primitive_TLV_inbound n + len_of_asn1_primitive_TLV_inbound s);
-  (* Prf *) assert (asn1_length_inbound_of_type SEQUENCE (Seq.length (serialize serialize_inner_value x)));
-  (* Prf *) assert (length_of_asn1_primitive_TLV n + length_of_asn1_primitive_TLV s == length_of_inner_t_value x);
-
-  (* Prf *) serialize_asn1_sequence_value_unfold
-              serialize_inner_value
-              (parser_tag_of_asn1_sequence serialize_inner_value x)
-              x;
-
-  (* Prf *) assert ((serialize serialize_inner_sequence x) `Seq.equal`
-                    ( (serialize (serialize_the_asn1_tag SEQUENCE) SEQUENCE)
-                    `Seq.append` (serialize (serialize_asn1_length_of_type SEQUENCE) (len_of_inner_t_inbound x))
-                    `Seq.append` (serialize (serialize_inner_value) x) ));
-
-  (* Prf *) assert (Seq.length (serialize serialize_inner_sequence x) ==
-                    ( Seq.length (serialize (serialize_the_asn1_tag SEQUENCE) SEQUENCE)
-                    + Seq.length (serialize (serialize_asn1_length_of_type SEQUENCE) (len_of_inner_t_inbound x))
-                    + Seq.length (serialize (serialize_inner_value) x) ));
-  (* Prf *) assert (Seq.length (serialize serialize_inner_sequence x) ==
-                    ( 1
-                    + v (len_of_asn1_length (len_of_inner_t_inbound x))
-                    + length_of_inner_t_value x ));
-
-  (* Finally... *)
-  (* Prf *) assert (Seq.length (serialize serialize_inner_sequence x) <= v pos /\ v pos <= B.length dst);
-
-  (* NOTE: Serialization. *)
-  (* Prf *) writable_weaken
-            (* buf *) dst
-            (*range*) 0 (B.length dst)
-            (* mem *) h0
-            (* from*) (v pos - length_of_inner_t_value x)
-            (* to  *) (v pos);
-
-  let offset = serialize32_inner_sequence_backwards
-               (*val*) x
-               (*dst*) dst
-               (*pos*) pos in
-
-  (* NOTE: Reason about the content of serialization. *)
-  (* Prf *) let h1 = HST.get () in
-  (* Prf *) assert (B.modifies (B.loc_buffer_from_to dst (pos - offset) pos) h0 h1);
-  (* Prf *) assert (serialize serialize_inner_sequence x
-                    `Seq.equal`
-                    Seq.slice (B.as_seq h1 dst) (v (pos - offset)) (v pos));
-
-  HST.pop_frame ()
-#pop-options
-
-
-
-open FStar.Tactics
-
-#push-options "--query_stats --z3rlimit 32"
-
-let rec gen_asn1_primitive_TLV_parser_kind
-  (l: list asn1_primitive_type)
-: parser_kind
-= match l with
-  | a1 :: l' -> (parse_asn1_TLV_kind_of_type a1
-                `and_then_kind`
-                gen_asn1_primitive_TLV_parser_kind l')
-  | []      -> (parse_ret_kind)
-
-let rec gen_asn1_primitive_TLV_parser_type
-  (l: list asn1_primitive_type)
-: Type0
-= match l with
-  | a1 :: l' -> (datatype_of_asn1_type a1 & gen_asn1_primitive_TLV_parser_type l')
-  | []      -> unit
-
-let rec gen_asn1_primitive_TLV_parser
-  (l: list asn1_primitive_type)
-: parser (gen_asn1_primitive_TLV_parser_kind l) (gen_asn1_primitive_TLV_parser_type l)
-= match l with
-  | a1 :: l' -> (parse_asn1_TLV_of_type a1
-                `nondep_then`
-                gen_asn1_primitive_TLV_parser l')
-  | []      -> (parse_ret ())
-
-let c = gen_asn1_primitive_TLV_parser [NULL; NULL; NULL; BOOLEAN]
-
-type test_t =
-| Test_t: (a: datatype_of_asn1_type NULL) -> (b: datatype_of_asn1_type OCTET_STRING) -> test_t
-
-let inspect_test
-  (se: sigelt)
-: Tac unit
-= let (.[]) = List.Tot.index in
-  let r = lookup_typ (top_env ()) ["test_t"] in
-    guard (Some? r);
-  let Some se = r in
-  let sv = inspect_sigelt se in
-    guard (Sg_Inductive? sv);
-  let Sg_Inductive name us params ty constructors = sv in
-    guard (List.length constructors = 1);
-
-  let constructor_r = lookup_typ (top_env ()) constructors.[0] in
-    guard (Some? constructor_r);
-  let constructor_sv = inspect_sigelt (Some?.v constructor_r) in
-    guard (Sg_Constructor? constructor_sv);
-  let Sg_Constructor name typ = constructor_sv in
-  let indices = inspect_ln typ in
-  _ by (dump "inspect"; exact (`()))
