src/asn1/ASN1.Base.fst
@@ -8,11 +8,11 @@ let lbytes = Seq.Properties.lseq byte
 
 type asn1_type: Type =
 | BOOLEAN
-// | INTEGER
+| INTEGER
 | NULL
 | OCTET_STRING
-// | BIT_STRING
-// | OID
+| BIT_STRING
+| OID
 | SEQUENCE
 
 let the_asn1_type (a: asn1_type)
@@ -32,19 +32,25 @@ let asn1_length_min_of_type
   (a: asn1_type)
 : asn1_length_t
 = match a with
-  | BOOLEAN   -> 1
-  | NULL -> 0
+  | BOOLEAN      -> 1
+  | INTEGER      -> 1
+  | NULL         -> 0
   | OCTET_STRING -> asn1_length_min
-  | SEQUENCE -> asn1_length_min
+  | OID          -> asn1_length_min
+  | BIT_STRING   -> 1
+  | SEQUENCE     -> asn1_length_min
 
 let asn1_length_max_of_type
   (a: asn1_type)
 : asn1_length_t
 = match a with
-  | BOOLEAN   -> 1
-  | NULL -> 0
+  | BOOLEAN      -> 1
+  | INTEGER      -> 4
+  | NULL         -> 0
   | OCTET_STRING -> asn1_length_max
-  | SEQUENCE -> asn1_length_max
+  | OID          -> asn1_length_max
+  | BIT_STRING   -> asn1_length_max
+  | SEQUENCE     -> asn1_length_max
 
 let asn1_length_bound_of_type
   (a: asn1_type)
@@ -56,6 +62,10 @@ let asn1_length_inbound_of_type
 : bool
 = let min, max = asn1_length_bound_of_type a in
   asn1_length_inbound x min max
+
+let asn1_length_of_type
+  (a: asn1_type)
+= l: asn1_length_t {asn1_length_inbound_of_type a l}
 
 let asn1_int32 = LowParse.Spec.BoundedInt.bounded_int32 asn1_length_min asn1_length_max
 let asn1_int32_min: i: asn1_int32 {forall (i': asn1_int32). i <= i'} = 0ul
@@ -70,19 +80,25 @@ let asn1_int32_min_of_type
   (a: asn1_type)
 : asn1_int32
 = match a with
-  | BOOLEAN   -> 1ul
-  | NULL -> 0ul
+  | BOOLEAN      -> 1ul
+  | INTEGER      -> 4ul
+  | NULL         -> 0ul
   | OCTET_STRING -> asn1_int32_min
-  | SEQUENCE -> asn1_int32_min
+  | OID          -> asn1_int32_min
+  | BIT_STRING   -> asn1_int32_min
+  | SEQUENCE     -> asn1_int32_min
 
 let asn1_int32_max_of_type
   (a: asn1_type)
 : asn1_int32
 = match a with
-  | BOOLEAN   -> 1ul
-  | NULL -> 0ul
+  | BOOLEAN      -> 1ul
+  | INTEGER      -> 5ul
+  | NULL         -> 0ul
   | OCTET_STRING -> asn1_int32_max
-  | SEQUENCE -> asn1_int32_max
+  | OID          -> asn1_int32_max
+  | BIT_STRING   -> asn1_int32_max
+  | SEQUENCE     -> asn1_int32_max
 
 let asn1_int32_bound_of_type
   (a: asn1_type)
@@ -96,40 +112,62 @@ let weak_kind_of_type
 = let min, max = asn1_length_bound_of_type a in
   LowParse.Spec.Base.strong_parser_kind min max None
 
+(* FStar.Integers does not have `lognot` *)
+
+type oid_t =
+| RIOT_OID
+| ECDSA_WITH_SHA256_OID
+| KEY_USAGE_OID
+
 ///
 unfold
 let datatype_of_asn1_type (a: asn1_primitive_type): Type
 = match a with
-  | BOOLEAN -> bool
-  | NULL -> unit
-  | OCTET_STRING -> (len: asn1_int32_of_type OCTET_STRING & s: bytes {Seq.length s == v len})
+  | BOOLEAN      -> bool
+  | INTEGER      -> uint_32
+  | NULL         -> unit
+  | OCTET_STRING -> ( len: asn1_int32_of_type OCTET_STRING &
+                      s  : bytes { Seq.length s == v len } )
+  | OID          -> oid_t
+  | BIT_STRING   -> ( bits: nat {0 <= bits /\ bits <= normalize_term ((asn1_length_max - 1) * 8)} &
+                      s  : bytes { let bytes_length: l:asn1_length_t {l <= asn1_length_max - 1} = normalize_term ((bits + 7) / 8) in
+                                   let unused_bits: n:nat{0 <= n /\ n <= 7} = normalize_term ((bytes_length * 8) - bits) in
+                                   Seq.length s == bytes_length /\
+                                  (if bytes_length = 0 then
+                                   ( bits == 0 )
+                                   else
+                                   ( let mask: n:nat{cast_ok (Unsigned W8) n} = normalize_term (pow2 unused_bits) in
+                                     0 == normalize_term ((v s.[bytes_length - 1]) % mask) ))} )
 
-type asn1_value: Type =
-| BOOLEAN_VALUE: b: bool -> asn1_value
-| NULL_VALUE: n: unit -> asn1_value
-| OCTET_STRING_VALUE: len: asn1_int32_of_type OCTET_STRING (* NOTE: Carrying length here for low-level operations. *)
-                   -> s: bytes{v len == Seq.length s}
-                   -> asn1_value
+// type asn1_value: Type =
+// | BOOLEAN_VALUE: b: bool -> asn1_value
+// | NULL_VALUE: n: unit -> asn1_value
+// | OCTET_STRING_VALUE: len: asn1_int32_of_type OCTET_STRING (* NOTE: Carrying length here for low-level operations. *)
+//                    -> s: bytes{v len == Seq.length s}
+//                    -> asn1_value
 
-unfold
-let asn1_value_of_type (a: asn1_primitive_type): Type
-= match a with
-  | BOOLEAN      -> value: asn1_value{BOOLEAN_VALUE? value}
-  | NULL         -> value: asn1_value{NULL_VALUE? value}
-  | OCTET_STRING -> value: asn1_value{OCTET_STRING_VALUE? value}
+// unfold
+// let asn1_value_of_type (a: asn1_primitive_type): Type
+// = match a with
+//   | BOOLEAN      -> value: asn1_value{BOOLEAN_VALUE? value}
+//   | NULL         -> value: asn1_value{NULL_VALUE? value}
+//   | OCTET_STRING -> value: asn1_value{OCTET_STRING_VALUE? value}
 
-let asn1_boolean = value: asn1_value{BOOLEAN_VALUE? value}
-let asn1_null = value: asn1_value{NULL_VALUE? value}
-let asn1_octet_string = value: asn1_value{OCTET_STRING_VALUE? value}
+// let asn1_boolean = value: asn1_value{BOOLEAN_VALUE? value}
+// let asn1_null = value: asn1_value{NULL_VALUE? value}
+// let asn1_octet_string = value: asn1_value{OCTET_STRING_VALUE? value}
 
-// let len_of_asn1_data
-//   (_a: asn1_primitive_type)
-//   (x: datatype_of_asn1_type _a)
-// : Tot (asn1_int32_of_type _a)
-// = match _a with
-//   | BOOLEAN      -> 1ul
-//   | NULL         -> 0ul
-//   | OCTET_STRING -> dfst (x <: datatype_of_asn1_type OCTET_STRING)
+let len_of_asn1_data
+  (_a: asn1_primitive_type)
+  (x: datatype_of_asn1_type _a)
+: Tot (asn1_int32_of_type _a)
+= match _a with
+  | BOOLEAN      -> 1ul
+  | INTEGER      -> admit()
+  | NULL         -> 0ul
+  | BIT_STRING   -> admit()//u (normalize_term ((dfst (x <: datatype_of_asn1_type BIT_STRING) + 7) / 8))
+  | OCTET_STRING -> dfst (x <: datatype_of_asn1_type OCTET_STRING)
+  | OID          -> admit()//dfst (x <: datatype_of_asn1_type OID)
 
 // let len_of_asn1_value
 //   (value: asn1_value)
