src/asn1/ASN1.Low.Test.fst
@@ -1,6 +1,6 @@
 module ASN1.Low.Test
 open ASN1.Base
-
+(*)
 open ASN1.Spec.Tag
 open ASN1.Spec.Length
 open ASN1.Spec.BOOLEAN
