src/asn1/ASN1.Spec.BITSTRING.fst
@@ -1,0 +1,239 @@
+module ASN1.Spec.BITSTRING
+
+open LowParse.Spec.Base
+open LowParse.Spec.Combinators
+open LowParse.Spec.SeqBytes.Base
+
+open ASN1.Base
+open ASN1.Spec.Tag
+open ASN1.Spec.Length
+
+open FStar.Integers
+
+/// TEST
+///
+
+// let bs_0: datatype_of_asn1_type BIT_STRING = (|0, Seq.empty|)
+// let bs_1: datatype_of_asn1_type BIT_STRING = (|1, Seq.create 1 128uy|)
+// let bs_2: datatype_of_asn1_type BIT_STRING = (|2, Seq.create 1 64uy|)
+// let bs_3: datatype_of_asn1_type BIT_STRING = (|3, Seq.create 1 32uy|)
+// let bs_4: datatype_of_asn1_type BIT_STRING = (|4, Seq.create 1 16uy|)
+// let bs_5: datatype_of_asn1_type BIT_STRING = (|5, Seq.create 1 8uy|)
+// let bs_6: datatype_of_asn1_type BIT_STRING = (|6, Seq.create 1 4uy|)
+// let bs_7: datatype_of_asn1_type BIT_STRING = (|7, Seq.create 1 2uy|)
+// let bs_8: datatype_of_asn1_type BIT_STRING = (|8, Seq.create 1 1uy|)
+// let bs_9: datatype_of_asn1_type BIT_STRING = (|9, Seq.create 2 128uy|)
+
+(*
+   Len = 1, unused = 0, bytes = []
+   Len = 2, unused = x, bytes = [_]
+*)
+
+let filter_asn1_bit_string
+  (l: asn1_length_of_type BIT_STRING)
+  (ls: lbytes l)
+: GTot (bool)
+= let unused_bits = ls.[0] in
+  if l = 1 then
+  ( unused_bits = 0uy )
+  else
+  ( let mask = normalize_term (pow2 (v unused_bits)) in
+    unused_bits <= 7uy && 0 = normalize_term ((v ls.[l - 1]) % mask) )
+
+let synth_asn1_bit_string
+  (l: asn1_length_of_type BIT_STRING)
+  (ls: parse_filter_refine (filter_asn1_bit_string l))
+: GTot (x: datatype_of_asn1_type BIT_STRING {
+           let (|bits, s|) = x in
+           let bytes_length = normalize_term ((bits + 7) / 8) in
+           let unused_bits = normalize_term ((bytes_length * 8) - bits) in
+           v ls.[0] == unused_bits /\
+           l == bytes_length + 1 })
+= let unused_bits = ls.[0] in
+  let s = Seq.slice ls 1 l in
+  if l = 1 then
+  ( assert_norm ( v unused_bits == 0 )
+  ; let bits: n:nat{n == 0} = normalize_term ((l - 1) * 8 - (v unused_bits)) in
+    (|bits, s|) )
+  else
+  ( assert_norm ( v unused_bits <= 7 )
+  ; let bits: n:nat {
+        0 <= n /\
+        n <= normalize_term ((asn1_length_max - 1) * 8)
+    } = normalize_term ((l - 1) * 8 - (v unused_bits)) in
+    (|bits, s|) )
+
+#push-options "--query_stats --z3rlimit 16"
+let synth_asn1_bit_string_injective'
+  (l: asn1_length_of_type BIT_STRING)
+  (ls1 ls2: parse_filter_refine (filter_asn1_bit_string l))
+: Lemma
+  (requires synth_asn1_bit_string l ls1 == synth_asn1_bit_string l ls2)
+  (ensures ls1 `Seq.equal` ls2)
+=
+  let unused_bits1 = ls1.[0] in
+  let unused_bits2 = ls2.[0] in
+  let s1 = Seq.slice ls1 1 l in
+  let s2 = Seq.slice ls2 1 l in
+  assert_norm ((unused_bits1 `Seq.cons` s1) `Seq.equal` ls1);
+  assert_norm ((unused_bits2 `Seq.cons` s2) `Seq.equal` ls2);
+  if l = 1 then
+  ( assert_norm (unused_bits1 == unused_bits2) )
+  else
+  ( let bits1: n:nat {
+        0 <= n /\
+        n <= normalize_term ((asn1_length_max - 1) * 8)
+    } = normalize_term ((l - 1) * 8 - (v unused_bits1)) in
+    let bits2: n:nat {
+        0 <= n /\
+        n <= normalize_term ((asn1_length_max - 1) * 8)
+    } = normalize_term ((l - 1) * 8 - (v unused_bits2)) in
+    assert_norm (bits1 == bits2)
+  ; assert_norm (unused_bits1 == unused_bits2)
+  ; assert_norm (s1 `Seq.equal` s2)
+  ; assert_norm ((unused_bits1 `Seq.cons` s1) `Seq.equal` ls1)
+  ; assert_norm ((unused_bits2 `Seq.cons` s2) `Seq.equal` ls2) )
+#pop-options
+
+let synth_asn1_bit_string_injective
+  (l: asn1_length_of_type BIT_STRING)
+: Lemma (
+  synth_injective (synth_asn1_bit_string l)
+)
+= synth_injective_intro' (synth_asn1_bit_string l) (synth_asn1_bit_string_injective' l)
+
+let synth_asn1_bit_string_inverse
+  (l: asn1_length_of_type BIT_STRING)
+  (x: datatype_of_asn1_type BIT_STRING {
+           let (|bits, s|) = x in
+           let bytes_length = normalize_term ((bits + 7) / 8) in
+           let unused_bits = normalize_term ((bytes_length * 8) - bits) in
+           l == bytes_length + 1 })
+: GTot (ls: parse_filter_refine (filter_asn1_bit_string l) { x == synth_asn1_bit_string l ls })
+= let (|bits, s|) = x in
+  let bytes_length: l:asn1_length_t { l <= asn1_length_max - 1 } = l - 1 in
+  let unused_bits: n:nat{0 <= n /\ n <= 7} = normalize_term ((bytes_length * 8) - bits) in
+  assert (Seq.length s == bytes_length);
+  let ls: parse_filter_refine (filter_asn1_bit_string l)
+      = normalize_term (Seq.create 1 (u unused_bits) `Seq.append` s) in
+  assert_norm (bytes_length == 0 ==>
+                 unused_bits == 0);
+  assert_norm (bytes_length <> 0 ==>
+                 unused_bits <= 7 /\
+                (bytes_length * 8 - unused_bits == bits));
+  assert (Seq.slice ls 1 l `Seq.equal` s);
+  assert (x == synth_asn1_bit_string l ls);
+  ls
+
+let parse_asn1_bit_string
+  (l: asn1_length_of_type BIT_STRING)
+: parser _ (x: datatype_of_asn1_type BIT_STRING {
+               let (|bits, s|) = x in
+               let bytes_length = normalize_term ((bits + 7) / 8) in
+               let unused_bits = normalize_term ((bytes_length * 8) - bits) in
+               l == bytes_length + 1 })
+= synth_asn1_bit_string_injective l;
+  parse_seq_flbytes l
+  `parse_filter`
+  filter_asn1_bit_string l
+  `parse_synth`
+  synth_asn1_bit_string l
+
+#push-options "--query_stats --z3rlimit 16 --lax"
+let parse_asn1_bit_string_unfold
+  (l: asn1_length_of_type BIT_STRING)
+  (input: bytes)
+: Lemma (
+  parse (parse_asn1_bit_string l) input ==
+ (match parse (parse_seq_flbytes l) input with
+  | None -> None
+  | Some (ls, consumed) -> ( if filter_asn1_bit_string l ls then
+                             ( Some (synth_asn1_bit_string l ls, consumed) )
+                             else
+                             ( None )))
+)
+= parse_filter_eq
+  (* p *) (parse_seq_flbytes l)
+  (* f *) (filter_asn1_bit_string l)
+  (* in*) (input);
+  synth_asn1_bit_string_injective l;
+  parse_synth_eq
+  (* p *) (parse_seq_flbytes l
+           `parse_filter`
+           filter_asn1_bit_string l)
+  (* f *) (synth_asn1_bit_string l)
+  (* in*) (input)
+#pop-options
+
+let serialize_asn1_bit_string
+  (l: asn1_length_of_type BIT_STRING)
+: serializer (parse_asn1_bit_string l)
+= serialize_synth
+  (* p1 *) (parse_seq_flbytes l
+            `parse_filter`
+            filter_asn1_bit_string l)
+  (* f2 *) (synth_asn1_bit_string l)
+  (* s1 *) (serialize_seq_flbytes l
+            `serialize_filter`
+            filter_asn1_bit_string l)
+  (* g1 *) (synth_asn1_bit_string_inverse l)
+  (* prf*) (synth_asn1_bit_string_injective l)
+
+let parser_tag_of_bit_string
+  (x: datatype_of_asn1_type BIT_STRING)
+: GTot (the_asn1_type BIT_STRING & asn1_int32_of_type BIT_STRING)
+= let (|bits, s|) = x in
+  let bytes_length = normalize_term ((bits + 7) / 8) in
+  let len: asn1_int32_of_type BIT_STRING = u (bytes_length + 1) in
+  (BIT_STRING, len)
+
+let synth_asn1_bit_string_TLV
+  (tag: (the_asn1_type BIT_STRING & asn1_int32_of_type BIT_STRING))
+  (value: datatype_of_asn1_type BIT_STRING {
+          let (|bits, s|) = value in
+          let bytes_length = normalize_term ((bits + 7) / 8) in
+          let unused_bits = normalize_term ((bytes_length * 8) - bits) in
+          v (snd tag) == bytes_length + 1 })
+: GTot (value': refine_with_tag parser_tag_of_bit_string tag)
+= value
+
+let synth_asn1_bit_string_TLV_inverse
+  (tag: (the_asn1_type BIT_STRING & asn1_int32_of_type BIT_STRING))
+  (value': refine_with_tag parser_tag_of_bit_string tag)
+: GTot (value: datatype_of_asn1_type BIT_STRING {
+               let (|bits, s|) = value in
+               let bytes_length = normalize_term ((bits + 7) / 8) in
+               let unused_bits = normalize_term ((bytes_length * 8) - bits) in
+               v (snd tag) == bytes_length + 1 /\
+               value' == synth_asn1_bit_string_TLV tag value})
+= value'
+
+let parse_asn1_bit_string_TLV
+= parse_tagged_union
+  (* pt *) (parse_the_asn1_tag BIT_STRING
+            `nondep_then`
+            parse_asn1_length_of_type BIT_STRING)
+  (* tg *) (parser_tag_of_bit_string)
+  (* p  *) (fun parser_tag -> weak_kind_of_type BIT_STRING
+                            `weaken`
+                           (parse_asn1_bit_string (v (snd parser_tag))
+                            `parse_synth`
+                            synth_asn1_bit_string_TLV parser_tag))
+
+#push-options "--query_stats --initial_fuel 4"
+let serialize_asn1_bit_string_TLV
+: serializer parse_asn1_bit_string_TLV
+= serialize_tagged_union
+  (* st *) (serialize_the_asn1_tag BIT_STRING
+            `serialize_nondep_then`
+            serialize_asn1_length_of_type BIT_STRING)
+  (* tg *) (parser_tag_of_bit_string)
+  (* s  *) (fun parser_tag -> weak_kind_of_type BIT_STRING
+                            `serialize_weaken`
+                           (serialize_synth
+                            (* p1 *) (parse_asn1_bit_string (v (snd parser_tag)))
+                            (* f2 *) (synth_asn1_bit_string_TLV parser_tag)
+                            (* s1 *) (serialize_asn1_bit_string (v (snd parser_tag)))
+                            (* g1 *) (synth_asn1_bit_string_TLV_inverse parser_tag)
+                            (* prf*) ()))
+#pop-options
