src/asn1/ASN1.Spec.TLV.Generic.fst
@@ -1,5 +1,5 @@
 module ASN1.Spec.TLV.Generic
-
+(*)
 open ASN1.Base
 open ASN1.Spec.Tag
 open ASN1.Spec.Length
