src/asn1/ASN1.Spec.TLV.Specialized.fst
@@ -1,5 +1,8 @@
 module ASN1.Spec.TLV.Specialized
 
+open LowParse.Spec.Base
+open LowParse.Spec.Combinators
+
 open ASN1.Base
 open ASN1.Spec.Tag
 open ASN1.Spec.Length
@@ -167,7 +170,7 @@ let len_of_asn1_primitive_TLV_inbound
 
 (* return *) tag_len + len_len + value_len
 #pop-options
-
+(*)
 /// Example
 ///
 type inner_t = {
